More reasonable proof of iter

zoo/hashtbl/lib/hashtbl.ml
@@ -1,18 +1,12 @@
-(* Based on:
-   https://github.com/ocaml-multicore/picos/blob/fa1da88bf3643fa18af2357a426e74ea2ac31072/lib/picos_aux.htbl/picos_aux_htbl.ml
-*)
+let[@zoo.opaque] eq _ _ = assert false
+let[@zoo.opaque] hash _ = assert false
 
-type ('k, 'v) bucket = 
-  | Nil 
-  | Cons of 'k * 'v * ('k, 'v) bucket
+type ('k, 'v) bucket = Nil | Cons of 'k * 'v * ('k, 'v) bucket
 
 type ('k, 'v) t = {
   mutable buckets : ('k, 'v) bucket array;
   mutable size : int;
 }
-
-let[@zoo.opaque] eq _ _ = assert false
-let[@zoo.opaque] hash _ = assert false
 
 let index k n = hash k mod n
 
@@ -25,24 +19,28 @@ let rec remove_assoc (k : 'k) (b : ('k, 'v) bucket) =
         let r, t = remove_assoc k t in
         (r, Cons (k', v, t))
 
-let create (n : int) = { 
-    buckets = Array.make n Nil;
-    size = 0 
-  }
+let create (n : int) = { buckets = Array.make n Nil; size = 0 }
 
-let add' (arr : (('k, 'v) bucket) array) (k : 'k) (v : 'v) =
+let add' (arr : ('k, 'v) bucket array) (k : 'k) (v : 'v) =
   let n = Array.size arr in
   let i = index k n in
-  arr.(i) <- Cons(k, v, arr.(i))
+  arr.(i) <- Cons (k, v, arr.(i))
 
 let rec bucket_iter_right (b : ('k, 'v) bucket) f : unit =
   match b with
-  |Nil -> ()
-  |Cons(k, v, b') ->
-    bucket_iter_right b' f;
-    f k v
+  | Nil -> ()
+  | Cons (k, v, b') ->
+      bucket_iter_right b' f;
+      f k v
 
-let iter (h : ('k, 'v) t) f =
-  for i = 0 to Array.size h.buckets - 1 do
-    bucket_iter_right h.buckets.(i) f
+let iter_aux (buckets : ('k, 'v) bucket array) f =
+  for i = 0 to Array.size buckets - 1 do
+    bucket_iter_right buckets.(i) f
   done
+
+let iter (h : ('k, 'v) t) f = iter_aux h.buckets f
+
+let resize (h : ('k, 'v) t) =
+  let len = Array.size h.buckets * 2 in
+  let new_buckets = Array.make len Nil in
+  iter_aux h.buckets (fun k v -> new_buckets.(index k len) <- v)
